Flapjack/Test/Backend.lean
@@ -10,6 +10,7 @@ import Flapjack.Test.AllocatorCalls
 import Flapjack.Test.AllocatorCorrectness
 import Flapjack.Test.AllocatorRegAlloc
 import Flapjack.Test.MustTerminate
+import Flapjack.Test.TailCalls
 import Flapjack.Test.WordToStack
 import Flapjack.Test.ParallelMove
 import Flapjack.Test.Stack
